pulse/ulib/experimental/Steel.Heap.fsti
@@ -399,28 +399,20 @@ let pre_action_with_frame
   (fp:slprop u#a)
   (a:Type u#b)
   (fp':a -> slprop u#a)
-  (frame:slprop u#a)
-  = full_hheap (fp `star` frame) -> (x:a & full_hheap (fp' x `star` frame))
-
-let post_preserves_frame_props
-  (#a: Type u#a)
-  (#fp: slprop u#b)
-  (#fp': a -> slprop u#b)
-  (frame:slprop u#b)
-  (f:pre_action_with_frame fp a fp' frame)
-  =
-  forall (h0:full_hheap (fp `star` frame)).
-     (let (| x, h1 |) = f h0 in
-      heap_evolves h0 h1 /\
-      (forall ctr. h0 `free_above_addr` ctr ==> h1 `free_above_addr` ctr) /\
-      (forall (hp:hprop frame). hp h0 == hp h1))
+  = frame:slprop u#a ->
+    full_hheap (fp `star` frame) -> (x:a & full_hheap (fp' x `star` frame))
 
 let action_with_frame
   (fp:slprop u#b)
   (a:Type u#a)
   (fp':a -> slprop u#b)
-  (frame:slprop u#b)
-  = f:pre_action_with_frame fp a fp' frame{post_preserves_frame_props frame f}
+  = f:(pre_action_with_frame fp a fp'){
+      forall (frame:slprop u#b)
+        (h0:full_hheap (fp `star` frame)).
+        (let (| x, h1 |) = f frame h0 in
+         heap_evolves h0 h1 /\
+         (forall ctr. h0 `free_above_addr` ctr ==> h1 `free_above_addr` ctr) /\
+         (forall (hp:hprop frame). hp h0 == hp h1))}
 
 (**
   Two heaps [h0] and [h1] are frame-related if you can get from [h0] to [h1] with a
